# 1.1
## 1.1.a)
We consider the following function

$$J(v)=\int_{-\pi}^{\pi} x^2 |v(x)+1|^2 dx$$

with $v$ piecewise $v \in C_{pw}^{0}([-\pi,\pi])$; thus we can start to solve the integral as

$$ \begin{align}
J(v) &=\int_{-\pi}^{\pi} x^2 |v(x)+1|^2 dx \\
&= \int_{-\pi}^{\pi} x^2 (v(x)^2+2v(x)+1) dx \\
&= \int_{-\pi}^{\pi} x^2v(x)^2 dx + \int_{-\pi}^{\pi}2x^2v(x) dx + \int_{-\pi}^{\pi}x^2dx \\
&=\ int_{-\pi}^{\pi} x^2v(x)^2 dx + \int_{-\pi}^{\pi}2x^2v(x) dx + \dfrac{2}{3}\pi^3 \\
&=\ int_{-\pi}^{\pi} x^2v(x)^2 dx + \int_{-\pi}^{\pi}2x^2v(x) dx + \dfrac{2}{3}\pi^3 \\
&\Rightarrow \dfrac{1}{2} a(v,v) - l(v) + c\\
\end{align}
$$

Thus we get that $i)$, $ii)$ satisfied and we only need to analyse $a(v,v) ≥ 0$ the third point:

$$
a(v,v) = 2\int_{-\pi}^{\pi} x^2v(x)^2 dx ≥ 0
$$

and this is clearly positive given the two squares


## 1.1.b)
Consider $J(v)$ a function of the form

$$J(v)=\int_{-1}^{1} \dfrac{d^2}{dx^2}v(x) \dfrac{d}{dx}v(x) dx$$

with $v \in C^2([-1,1])$; we can then apply first the linear form with a second fuction $u(x)$

$$ \begin{align}
J(v) &= \int_{-1}^{1} \dfrac{d^2}{dx^2}v(x)u(x) \dfrac{d}{dx}v(x)u(x) dx \\
=& \int_{-1}^{1} \dfrac{d^2}{dx^2}v(x)\dfrac{d}{dx}u(x) + \dfrac{d^2}{dx^2}u(x)\dfrac{d}{dx}v(x) dx \\
\end{align}
$$

where we can state for the point $ii)$

$$ \begin{align}
a(u,v) &= \int_{-1}^{1} \dfrac{d^2}{dx^2}v(x)\dfrac{d}{dx}u(x) + \dfrac{d^2}{dx^2}u(x)\dfrac{d}{dx}v(x)\\
l(v) &= 0
\end{align}
$$

Finally it remains to see if $a$ is s.p.d.:

$$ \begin{align}
a(v,v) &= \int_{-1}^{1} \dfrac{d^2}{dx^2}v(x)\dfrac{d}{dx}v(x) + \dfrac{d^2}{dx^2}v(x)\dfrac{d}{dx}v(x)\\
&= 2\int_{-1}^{1}\dfrac{d^2}{dx^2}v(x)\dfrac{d}{dx}v(x)dx \\
&\Rightarrow v(x) = (x-1)^2 \\
&\Rightarrow  a(v,v) = 2\int_{-1}^{1}4(x-1)dx \\
&= -16 \\
\end{align} 
$$

and this proves that $a$ is not spd

## 1.1.d)
Be c a function of the following form:

$$J(v) = \int_{\Omega}|f(x)\cdot gradv-1|^2dx, \quad v\in C_{pw}^1(\Omega)$$

First we apply the binomial formula:

$$ \begin{align}
J(v) &= \int_{\Omega}|f(x)\cdot gradv-1|^2dx \\
&= \int_{\Omega}f(x)^2\cdot (gradv)^2-2f(x)\cdot (gradv)+1dx \\
&\Rightarrow a(u,v) = \int_{\Omega}f(x)^2\cdot [(gradv)(gradu)]dx, \\
&\quad \quad l(v) = -2\int_{\Omega}f(x)\cdot (gradv)dx \\
\end{align}
$$

Thus we only need to prove that $a(v,v)$ is s.p.d., given that we have a binomial form, we can directly say like in $a)$ that 

$$a(v,v) = \int_{\Omega}|f(x)\cdot gradv|^2dx ≥ 0$$

## 1.1.g)
Let $J(v)$ be equal to

$$J(v)= \dfrac{1}{2}a(v,v)-l(v)+c, \quad v\in V_0$$

and we first consider first

$$ \begin{align}
J(u+v)-J(u)-J(v)+J(0)&= \dfrac{1}{2}a(u+v,u+v)-l(u+v)+c-[\dfrac{1}{2}a(u,u)-l(u)+c]-[\dfrac{1}{2}a(v,v)-l(v)+c]+\dfrac{1}{2}a(0,0)-l(0)+c\\
&= \dfrac{1}{2}a(u+v,u+v)-l(u+v)-[\dfrac{1}{2}a(u,u)-l(u)]+\dfrac{1}{2}a(v,v)-l(v)] &(def. \quad 0.3.1.4)\\ 
&= \dfrac{1}{2}a(u,v)+\dfrac{1}{2}a(v,u)-l(u)-l(v)+l(u)+l(v)] &(def. \quad 0.3.1.15)\\ 
&= a(u,v)\\
\end{align}
$$